%%%%%%%%%%%%%%%%%%%%%%%%%%%%%%%%%%%%%%%%%
% LaTeX Template
% http://www.LaTeXTemplates.com
%
% Original author:
% Linux and Unix Users Group at Virginia Tech Wiki 
% (https://vtluug.org/wiki/Example_LaTeX_chem_lab_report)
%
% License:
% CC BY-NC-SA 3.0 (http://creativecommons.org/licenses/by-nc-sa/3.0/)
%
%%%%%%%%%%%%%%%%%%%%%%%%%%%%%%%%%%%%%%%%%

%----------------------------------------------------------------------------------------
%	PACKAGES AND DOCUMENT CONFIGURATIONS
%----------------------------------------------------------------------------------------

\documentclass[11pt]{article}
\usepackage{geometry} % Pour passer au format A4
\geometry{hmargin=1cm, vmargin=1cm} % 

\usepackage{graphicx} % Required for including pictures
\usepackage{float} % 

%Français
\usepackage[T1]{fontenc} 
\usepackage[english,francais]{babel}
\usepackage[utf8]{inputenc}
\usepackage{eurosym}
\usepackage{lmodern}
\usepackage{url}
\usepackage{multicol}

%Maths
\usepackage{amsmath,amsfonts,amssymb,amsthm}
%\usepackage[linesnumbered, ruled, vlined]{algorithm2e}
%\SetAlFnt{\small\sffamily}

%Autres
\linespread{1} % Line spacing
\setlength\parindent{0pt} % Removes all indentation from paragraphs

\renewcommand{\labelenumi}{\alph{enumi}.} % 
\pagestyle{empty}

%----------------------------------------------------------------------------------------
%	DOCUMENT INFORMATION
%----------------------------------------------------------------------------------------
\begin{document}

%\maketitle % Insert the title, author and date

\setlength{\columnseprule}{1pt}

\begin{multicols}{3}
% ------ Exercice 1 ------
\section*{Dérivées}

\begin{eqnarray*}
f_{1}(x) &=& 12x^{15} - 5x^{12} - x^{8} - 2x^{4}\\
f_{2}(x) &=& 10x^{145} - 100x^{32} + 8^{1000}\\
f_{3}(x) &=& 3x^{-12} + x^{-6} - x^{-1}\\
f_{4}(x) &=& 4(x^{-6} - 2x^{-3} - x^{-1})\\
f_{5}(x) &=& -1024 (2x^{4} - 10x^{2} - x^{1})\\
f_{6}(x) &=& (3x^{2} - 2)^{4}\\
f_{7}(x) &=& (5x^{3} - 2x)^{11}\\
f_{8}(x) &=& (2x^{2} - 2x^{-4})^{7}\\
f_{9}(x) &=& x \times (2x^{2} - 2x)\\
f_{10}(x) &=& x^3 \times (-x^{2} + x) \\
f_{11}(x) &=& (x - 12) \times (-x^{2} + 6x)\\
f_{12}(x) &=& (x^3 + x) \times (2x^{3} + 9x)\\
f_{13}(x) &=& \frac{1}{3x + 1}\\
f_{14}(x) &=& \frac{1}{x^4 + 6}\\
f_{15}(x) &=& \frac{12}{x^2 - x}\\
f_{16}(x) &=& \frac{x}{x^3 - 2x}\\
f_{17}(x) &=& \frac{x^2 - 2x}{6x^4 - x}\\
f_{18}(x) &=& ln(x+1)\\
f_{19}(x) &=& ln(x^4 - 6x)\\
f_{20}(x) &=& x \times ln(-3x + 1)\\
f_{21}(x) &=& e^{2x +4}\\
f_{22}(x) &=& 5 e^{-4x^2 + 3x}\\
f_{23}(x) &=& x^4 \times e^{2x + 1}\\
f_{24}(x) &=& x^3 \times e^{x^4 - 2}\\
f_{25}(x) &=& 2 (x^2 - 3x) \times e^{-3x + 7}\\
f_{26}(x) &=& ln(x) \times e^{3x + 1}\\
f_{27}(x) &=& \frac{ln(3x+1)}{-4x+2}\\
f_{28}(x) &=& 8 \frac{2x-1}{e^{2x+1}}\\
f_{29}(x) &=& cos(2x+1)\\
f_{30}(x) &=& sin(-3x-3)\\
f_{31}(x) &=& cos(x) \times sin(x)\\
f_{32}(x) &=& cos(2x+1) \times sin(-3x)\\
f_{33}(x) &=& (cos(x) + x) \times e^{x}\\
f_{34}(x) &=& (sin(x) - x)^{4}\\
f_{35}(x) &=& \dfrac{cos(x)}{sin(x)}\\
f_{36}(x) &=& \ln(3x) \times sin(-3x)\\
\end{eqnarray*}

% ------ Exercice 1 ------
\section*{Dérivées}

\begin{eqnarray*}
f_{1}(x) &=& 12x^{15} - 5x^{12} - x^{8} - 2x^{4}\\
f_{2}(x) &=& 10x^{145} - 100x^{32} + 8^{1000}\\
f_{3}(x) &=& 3x^{-12} + x^{-6} - x^{-1}\\
f_{4}(x) &=& 4(x^{-6} - 2x^{-3} - x^{-1})\\
f_{5}(x) &=& -1024 (2x^{4} - 10x^{2} - x^{1})\\
f_{6}(x) &=& (3x^{2} - 2)^{4}\\
f_{7}(x) &=& (5x^{3} - 2x)^{11}\\
f_{8}(x) &=& (2x^{2} - 2x^{-4})^{7}\\
f_{9}(x) &=& x \times (2x^{2} - 2x)\\
f_{10}(x) &=& x^3 \times (-x^{2} + x) \\
f_{11}(x) &=& (x - 12) \times (-x^{2} + 6x)\\
f_{12}(x) &=& (x^3 + x) \times (2x^{3} + 9x)\\
f_{13}(x) &=& \frac{1}{3x + 1}\\
f_{14}(x) &=& \frac{1}{x^4 + 6}\\
f_{15}(x) &=& \frac{12}{x^2 - x}\\
f_{16}(x) &=& \frac{x}{x^3 - 2x}\\
f_{17}(x) &=& \frac{x^2 - 2x}{6x^4 - x}\\
f_{18}(x) &=& ln(x+1)\\
f_{19}(x) &=& ln(x^4 - 6x)\\
f_{20}(x) &=& x \times ln(-3x + 1)\\
f_{21}(x) &=& e^{2x +4}\\
f_{22}(x) &=& 5 e^{-4x^2 + 3x}\\
f_{23}(x) &=& x^4 \times e^{2x + 1}\\
f_{24}(x) &=& x^3 \times e^{x^4 - 2}\\
f_{25}(x) &=& 2 (x^2 - 3x) \times e^{-3x + 7}\\
f_{26}(x) &=& ln(x) \times e^{3x + 1}\\
f_{27}(x) &=& \frac{ln(3x+1)}{-4x+2}\\
f_{28}(x) &=& 8 \frac{2x-1}{e^{2x+1}}\\
f_{29}(x) &=& cos(2x+1)\\
f_{30}(x) &=& sin(-3x-3)\\
f_{31}(x) &=& cos(x) \times sin(x)\\
f_{32}(x) &=& cos(2x+1) \times sin(-3x)\\
f_{33}(x) &=& (cos(x) + x) \times e^{x}\\
f_{34}(x) &=& (sin(x) - x)^{4}\\
f_{35}(x) &=& \dfrac{cos(x)}{sin(x)}\\
f_{36}(x) &=& \ln(3x) \times sin(-3x)\\
\end{eqnarray*}

% ------ Exercice 1 ------
\section*{Dérivées}

\begin{eqnarray*}
f_{1}(x) &=& 12x^{15} - 5x^{12} - x^{8}-2x^{4}\\
f_{2}(x) &=& 10x^{145} - 100x^{32} + 8^{1000}\\
f_{3}(x) &=& 3x^{-12} + x^{-6} - x^{-1}\\
f_{4}(x) &=& 4(x^{-6} - 2x^{-3} - x^{-1})\\
f_{5}(x) &=& -1024 (2x^{4} - 10x^{2} - x^{1})\\
f_{6}(x) &=& (3x^{2} - 2)^{4}\\
f_{7}(x) &=& (5x^{3} - 2x)^{11}\\
f_{8}(x) &=& (2x^{2} - 2x^{-4})^{7}\\
f_{9}(x) &=& x \times (2x^{2} - 2x)\\
f_{10}(x) &=& x^3 \times (-x^{2} + x) \\
f_{11}(x) &=& (x - 12) \times (-x^{2} + 6x)\\
f_{12}(x) &=& (x^3 + x) \times (2x^{3} + 9x)\\
f_{13}(x) &=& \frac{1}{3x + 1}\\
f_{14}(x) &=& \frac{1}{x^4 + 6}\\
f_{15}(x) &=& \frac{12}{x^2 - x}\\
f_{16}(x) &=& \frac{x}{x^3 - 2x}\\
f_{17}(x) &=& \frac{x^2 - 2x}{6x^4 - x}\\
f_{18}(x) &=& ln(x+1)\\
f_{19}(x) &=& ln(x^4 - 6x)\\
f_{20}(x) &=& x \times ln(-3x + 1)\\
f_{21}(x) &=& e^{2x +4}\\
f_{22}(x) &=& 5 e^{-4x^2 + 3x}\\
f_{23}(x) &=& x^4 \times e^{2x + 1}\\
f_{24}(x) &=& x^3 \times e^{x^4 - 2}\\
f_{25}(x) &=& 2 (x^2 - 3x) \times e^{-3x + 7}\\
f_{26}(x) &=& ln(x) \times e^{3x + 1}\\
f_{27}(x) &=& \frac{ln(3x+1)}{-4x+2}\\
f_{28}(x) &=& 8 \frac{2x-1}{e^{2x+1}}\\
f_{29}(x) &=& cos(2x+1)\\
f_{30}(x) &=& sin(-3x-3)\\
f_{31}(x) &=& cos(x) \times sin(x)\\
f_{32}(x) &=& cos(2x+1) \times sin(-3x)\\
f_{33}(x) &=& (cos(x) + x) \times e^{x}\\
f_{34}(x) &=& (sin(x) - x)^{4}\\
f_{35}(x) &=& \dfrac{cos(x)}{sin(x)}\\
f_{36}(x) &=& \ln(3x) \times sin(-3x)\\
\end{eqnarray*}

\end{multicols}



\end{document}
