%%%%%%%%%%%%%%%%%%%%%%%%%%%%%%%%%%%%%%%%%
% LaTeX Template
% http://www.LaTeXTemplates.com
%
% Original author:
% Linux and Unix Users Group at Virginia Tech Wiki 
% (https://vtluug.org/wiki/Example_LaTeX_chem_lab_report)
%
% License:
% CC BY-NC-SA 3.0 (http://creativecommons.org/licenses/by-nc-sa/3.0/)
%
%%%%%%%%%%%%%%%%%%%%%%%%%%%%%%%%%%%%%%%%%

%----------------------------------------------------------------------------------------
%	PACKAGES AND DOCUMENT CONFIGURATIONS
%----------------------------------------------------------------------------------------

\documentclass[11pt]{article}
\usepackage{geometry} % Pour passer au format A4
\geometry{hmargin=1cm, vmargin=1cm} % 

\usepackage{graphicx} % Required for including pictures
\usepackage{float} % 

%Français
\usepackage[T1]{fontenc} 
\usepackage[english,francais]{babel}
\usepackage[utf8]{inputenc}
\usepackage{eurosym}
\usepackage{lmodern}
\usepackage{url}
\usepackage{multicol}

%Maths
\usepackage{amsmath,amsfonts,amssymb,amsthm}
%\usepackage[linesnumbered, ruled, vlined]{algorithm2e}
%\SetAlFnt{\small\sffamily}

%Autres
\linespread{1} % Line spacing
\setlength\parindent{0pt} % Removes all indentation from paragraphs

\renewcommand{\labelenumi}{\alph{enumi}.} % 
\pagestyle{empty}
%----------------------------------------------------------------------------------------
%	DOCUMENT INFORMATION
%----------------------------------------------------------------------------------------
\begin{document}

%\maketitle % Insert the title, author and date

\begin{minipage}[t]{\textwidth}
  \raggedright
      {\bfseries Série : \textbf{A}}\\
      {\bfseries BTS STS ET}\\[.35ex]
      \vspace*{-1cm}
      \raggedleft
          {\bfseries Complexes}\\[.35ex]
          {\bfseries 15 Septembre 2014}\\[.35ex]
\end{minipage}\\[1em]

\begin{center}
  \textsf{Yes, we’re being bought by Microsoft - Mojang - 2.5 Millards \$}\\
  \textsf{I’m leaving Mojang - It’s not about the money. It’s about my sanity. - Notch}
\end{center}

\setlength{\columnseprule}{1pt}

\begin{multicols}{2}

\section*{Série A}
    \subsection*{Données}
  \begin{eqnarray*}
    z_{0} & = & 2\\
    z_{1} & = & 3j\\
    z_{2} & = & j + 1\\
    z_{3} & = & 3(j+1)\\
    z_{4} & = & -2j\\
    z_{5} & = & -j + 1\\
    z_{6} & = & -j + 2\\
    z_{7} & = & 5\\
    z_{8} & = & -2j\\
    z_{9} & = & 2 + j\\
  \end{eqnarray*}

\section*{Série B}

  \subsection*{Données}

  \begin{eqnarray*}
    z_{0} & = & 1\\
    z_{1} & = & 2j\\
    z_{2} & = & j + 1\\
    z_{3} & = & 2(j+1)\\
    z_{4} & = & -4j\\
    z_{5} & = & -j - 1\\
    z_{6} & = & -j + 2\\
    z_{7} & = & 6\\
    z_{8} & = & -5j\\
    z_{9} & = & 2 + j\\
  \end{eqnarray*}
\end{multicols}

  \subsection*{Énoncés et solutions}
  \textbf{Calculer les expressions suivantes avec un résultat sous la forme $a + jb$ avec $a$, $b$ des réels et $j$ tel que $j^{2} = -1$.}

\begin{multicols}{2}

  \begin{enumerate}
  \item $z_{1} + z_{2} = 3j + (j+1) = 1 + 4j$
  \item $z_{0} - z_{3} + z_{2} = 2-3\times(j + 1) + (j + 1) = 2 - 3j -3 + j + 1= -2j$
  \item $z_{6}+ z_{1} + z_{4} = -j +2 + 3j + -2j = 2$
  \item $z_{7} \times z_{2} = 5\times (j+1) = 5 + 5j$
  \item $z_{2} + z_{7} \times z_{2} = j + 1 + (5 + 5j) = 6 + 6j$
  \item $(z_{2})^{2} = (j+1)^{2} = j^2 + 2\times j \times 1 + 1^2 = 1 + 2j - 1 = 2j$
  \item $(z_{1} + z_{2})^{2} = (1 + 4j)^2 = (4j)^2 + 2\times 1\times 4j + 1^2 = -16 + 8j + 1 = -15 + 8j$
  \item $\dfrac{1}{z_{1}} = \dfrac{1}{3j} = \dfrac{j}{-3} = -\dfrac{1}{3}\times j$
  \item $\dfrac{z_1}{z_5} = z_1 \times \dfrac{\overline{z_5}}{z_5 \overline{z_5}} = 3j \times \dfrac{1+j}{1^2 + 1^2} = 3j \times \dfrac{1+j}{2} = -\dfrac{3}{2} + \dfrac{3}{2}j$
  \item $\dfrac{z_9}{z_2} = z_9 \times \dfrac{\overline{z_2}}{z_2 \overline{z_2}} = (2+j) \times \dfrac{1-j}{2} = \dfrac{1}{2} \times \left( -2j + 2 + 1 + j \right) = \dfrac{3}{2} - \dfrac{1}{2}j$
  \end{enumerate}

  \begin{enumerate}
  \item $z_{1} + z_{2} = 2j + (j+1) = 1 + 3j$
  \item $z_{0} - z_{3} + z_{2} = 1 - 2\times(j + 1) + (j + 1) = 1 - 2j - 2 + j + 1 = -j$
  \item $z_{6}+ z_{1} + z_{4} = -j + 2 + 2j + -4j = 2 - 3j$
  \item $z_{7} \times z_{2} = 6\times (j+1) = 6 + 6j$
  \item $z_{2} + z_{7} \times z_{2} = j + 1 + (6 + 6j) = 7 + 7j$
  \item $(z_{2})^{2} = (j+1)^{2} = j^2 + 2\times j \times 1 + 1^2 = 1 + 2j - 1 = 2j$
  \item $(z_{1} + z_{2})^{2} = (1 + 3j)^2 = (3j)^2 + 2\times 1\times 3j + 1^2 = -9 + 6j + 1 = -8 + 6j$
  \item $\dfrac{1}{z_{1}} = \dfrac{1}{2j} = \dfrac{j}{-2} = -\dfrac{1}{2}\times j$
  \item $\dfrac{z_1}{z_5} = z_1 \times \dfrac{\overline{z_5}}{z_5 \overline{z_5}} = 2j \times \dfrac{-1-j}{1^2 + 1^2} = 2j \times \dfrac{-1-j}{2} = -1 - j$
  \item $\dfrac{z_9}{z_2} = z_9 \times \dfrac{\overline{z_2}}{z_2 \overline{z_2}} = (2+j) \times \dfrac{1-j}{2} = \dfrac{1}{2} \times \left( -2j + 2 + 1 + j \right) = \dfrac{3}{2} - \dfrac{1}{2}j$
  \end{enumerate}
\end{multicols}

\end{document}
